examples/n_german/nMutual.thy
@@ -3,6 +3,8 @@ theory nMutual
 begin
 
 
+subsection \<open>Definitions\<close>
+
 text \<open>Represents the four states: idle, try, critical, exit\<close>
 
 definition I :: scalrValueType where [simp]: "I \<equiv> enum ''control'' ''I''"
@@ -25,16 +27,6 @@ text \<open>Initial condition: x is True
 definition initSpec1 :: formula where
   "initSpec1 \<equiv> IVar (Ident ''x'') =\<^sub>f Const true"
 
-definition allInitSpecs :: "nat \<Rightarrow> formula list" where
-  "allInitSpecs N \<equiv> [initSpec0 N, initSpec1]"
-
-lemma absInitSpec:
-  assumes "M \<le> N"
-  shows "absTransfForm M (initSpec0 N) = initSpec0 M"
-        "absTransfForm M initSpec1 = initSpec1"
-  unfolding initSpec0_def initSpec1_def using assms by auto
-
-
 text \<open>There cannot be one state in exit and another in critical or exit.
   n[i] = E \<longrightarrow> (\<forall>j. i \<noteq> j \<longrightarrow> n[j] \<noteq> C \<and> n[j] \<noteq> E)
 \<close>
@@ -43,51 +35,80 @@ definition invAux :: "nat \<Rightarrow> nat \<Rightarrow> formula" where
                 forallFormExcl (\<lambda>j. \<not>\<^sub>f IVar (Para ''n'' j) =\<^sub>f Const C) i N \<and>\<^sub>f
                 forallFormExcl (\<lambda>j. \<not>\<^sub>f IVar (Para ''n'' j) =\<^sub>f Const E) i N"
 
-lemma symInvAux:
-  "symParamForm N (invAux N)"
-  unfolding invAux_def
-  apply (auto intro!: symParamFormImply symParamFormAnd symParamFormForall symParamFormForallExcl)
-  unfolding symParamForm_def symParamForm2_def equivForm_def by auto
-
-
 text \<open>Try enter critical region
   n[i] = I \<rightarrow> n[i] := T
 \<close>
 definition n_Try :: "nat \<Rightarrow> rule" where
   "n_Try i \<equiv>
-    let g = IVar (Para ''n'' i) =\<^sub>f Const I in
-    let s = assign (Para ''n'' i, Const T) in
-      guard g s"
+    IVar (Para ''n'' i) =\<^sub>f Const I
+   \<triangleright>
+    assign (Para ''n'' i, Const T)"
 
 text \<open>Enter critical region
   n[i] = T \<and> x = True \<rightarrow> n[i] := C; x := False
 \<close>
 definition n_Crit :: "nat \<Rightarrow> rule" where
   "n_Crit i \<equiv>
-    let g = IVar (Para ''n'' i) =\<^sub>f Const T \<and>\<^sub>f
-            IVar (Ident ''x'') =\<^sub>f Const true in
-    let s = assign (Para ''n'' i, Const C) ||
-            assign (Ident ''x'', Const false) in
-      guard g s"
+    IVar (Para ''n'' i) =\<^sub>f Const T \<and>\<^sub>f
+    IVar (Ident ''x'') =\<^sub>f Const true
+   \<triangleright>
+    assign (Para ''n'' i, Const C) ||
+    assign (Ident ''x'', Const false)"
 
 text \<open>Exit critical region
   n[i] = C \<rightarrow> n[i] := E
 \<close>
 definition n_Exit :: "nat \<Rightarrow> rule" where
   "n_Exit i \<equiv>
-    let g = IVar (Para ''n'' i) =\<^sub>f Const C in
-    let s = assign (Para ''n'' i, Const E) in
-      guard g s"
+    IVar (Para ''n'' i) =\<^sub>f Const C
+   \<triangleright>
+    assign (Para ''n'' i, Const E)"
 
 text \<open>Move to idle
   n[i] = E \<rightarrow> n[i] := I; x := True
 \<close>
 definition n_Idle :: "nat \<Rightarrow> rule" where
   "n_Idle i \<equiv>
-    let g = IVar (Para ''n'' i) =\<^sub>f Const E in
-    let s = assign (Para ''n'' i, Const I) ||
-            assign (Ident ''x'', Const true) in
-      guard g s"
+    IVar (Para ''n'' i) =\<^sub>f Const E
+   \<triangleright>
+    assign (Para ''n'' i, Const I) ||
+    assign (Ident ''x'', Const true)"
+
+definition n_Idle2 :: "nat \<Rightarrow> nat \<Rightarrow> rule" where
+  "n_Idle2 N i = strengthenRule2 (invAux N i) (n_Idle i)"
+
+subsection \<open>References\<close>
+
+definition n_Crit_abs :: rule where
+  "n_Crit_abs \<equiv>
+    IVar (Ident ''x'') =\<^sub>f Const (boolV True)
+   \<triangleright>
+    assign (Ident ''x'', Const (boolV False))"
+
+definition n_Idle_abs1 :: rule where
+  "n_Idle_abs1 \<equiv>
+    chaos \<triangleright> assign (Ident ''x'', Const true)"
+
+definition n_Idle_abs2 :: "nat \<Rightarrow> rule" where
+  "n_Idle_abs2 M \<equiv>
+    (\<forall>\<^sub>fj. \<not>\<^sub>f IVar (Para ''n'' j) =\<^sub>f Const (enum ''control'' ''C'')) M \<and>\<^sub>f
+    (\<forall>\<^sub>fj. \<not>\<^sub>f IVar (Para ''n'' j) =\<^sub>f Const (enum ''control'' ''E'')) M
+   \<triangleright>
+    assign (Ident ''x'', Const (boolV True))"
+
+subsection \<open>Individual tests\<close>
+
+lemma absInitSpec:
+  assumes "M \<le> N"
+  shows "absTransfForm M (initSpec0 N) = initSpec0 M"
+        "absTransfForm M initSpec1 = initSpec1"
+  unfolding initSpec0_def initSpec1_def using assms by auto
+
+lemma symInvAux:
+  "symParamForm N (invAux N)"
+  unfolding invAux_def
+  apply (auto intro!: symParamFormImply symParamFormAnd symParamFormForall symParamFormForallExcl)
+  unfolding symParamForm_def symParamForm2_def equivForm_def by auto
 
 lemma symTry:
   "symParamRule N n_Try"
@@ -105,7 +126,7 @@ lemma symIdle:
   "symParamRule N n_Idle"
   unfolding n_Idle_def symParamRule_def by auto
 
-lemma absTry:
+lemma absTryGuard:
   "absTransfForm M (pre (n_Try i)) =
     (if i > M then
        dontCareForm
@@ -121,7 +142,12 @@ lemma absTryAct:
        assign (Para ''n'' i, Const T))"
   unfolding n_Try_def by auto
 
-lemma absCrit:
+lemma absTry:
+  "absTransfRule M (n_Try i) =
+    (if i \<le> M then n_Try i else chaos \<triangleright> skip)"
+  by (auto simp add: n_Try_def)
+
+lemma absCritGuard:
   "absTransfForm M (pre (n_Crit i)) =
     (if i > M then
        IVar (Ident ''x'') =\<^sub>f Const (boolV True)
@@ -139,7 +165,12 @@ lemma absCritAct:
        assign (Ident ''x'', Const false))"
   unfolding n_Crit_def by auto
 
-lemma absExit:
+lemma absCrit:
+  "absTransfRule M (n_Crit i) =
+   (if i \<le> M then n_Crit i else n_Crit_abs)"
+  unfolding n_Crit_def n_Crit_abs_def by auto
+
+lemma absExitGuard:
   "absTransfForm M (pre (n_Exit i)) =
     (if i > M then
        dontCareForm
@@ -155,7 +186,12 @@ lemma absExitAct:
        assign (Para ''n'' i, Const E))"
   unfolding n_Exit_def by auto
 
-lemma absIdle:
+lemma absExit:
+  "absTransfRule M (n_Exit i) =
+   (if i \<le> M then n_Exit i else chaos \<triangleright> skip)"
+  unfolding n_Exit_def by auto
+
+lemma absIdleGuard:
   "absTransfForm M (pre (n_Idle i)) =
     (if i > M then
        dontCareForm
@@ -172,12 +208,14 @@ lemma absIdleAct:
        assign (Ident ''x'', Const true))"
   unfolding n_Idle_def by auto
 
-definition n_Idle_st :: "nat \<Rightarrow> nat \<Rightarrow> rule" where
-  "n_Idle_st N i = strengthenRule2 (invAux N i) (n_Idle i)"
+lemma absIdle:
+  "absTransfRule M (n_Idle i) =
+   (if i \<le> M then n_Idle i else n_Idle_abs1)"
+  unfolding n_Idle_def n_Idle_abs1_def by auto
 
 lemma symIdle2:
-  "symParamRule N (n_Idle_st N)" 
-  unfolding n_Idle_st_def
+  "symParamRule N (n_Idle2 N)" 
+  unfolding n_Idle2_def
   by (auto intro!: symParamStrengthenRule2 symIdle symInvAux)
 
 text \<open>Move to idle, strengthened:
@@ -185,29 +223,35 @@ text \<open>Move to idle, strengthened:
   (\<forall>j. i \<noteq> j \<longrightarrow> n[j] \<noteq> C) \<and>
   (\<forall>j. i \<noteq> j \<longrightarrow> n[j] \<noteq> E) \<rightarrow> n[i] := I; x := True
 \<close>
-definition n_Idle_st_ref :: "nat \<Rightarrow> nat \<Rightarrow> rule" where
-  "n_Idle_st_ref N i \<equiv>
-    let g = IVar (Para ''n'' i) =\<^sub>f Const E \<and>\<^sub>f
-            forallFormExcl (\<lambda>j. \<not>\<^sub>f IVar (Para ''n'' j) =\<^sub>f Const C) i N \<and>\<^sub>f
-            forallFormExcl (\<lambda>j. \<not>\<^sub>f IVar (Para ''n'' j) =\<^sub>f Const E) i N in
-    let a = assign (Para ''n'' i, Const I) ||
-            assign (Ident ''x'', Const true) in
-      guard g a"
+definition n_Idle2_ref :: "nat \<Rightarrow> nat \<Rightarrow> rule" where
+  "n_Idle2_ref N i \<equiv>
+    IVar (Para ''n'' i) =\<^sub>f Const E \<and>\<^sub>f
+    forallFormExcl (\<lambda>j. \<not>\<^sub>f IVar (Para ''n'' j) =\<^sub>f Const C) i N \<and>\<^sub>f
+    forallFormExcl (\<lambda>j. \<not>\<^sub>f IVar (Para ''n'' j) =\<^sub>f Const E) i N
+   \<triangleright>
+    assign (Para ''n'' i, Const I) ||
+    assign (Ident ''x'', Const true)"
 
-lemma n_Idle_stEq:
-  "n_Idle_st N i = n_Idle_st_ref N i"
-  by (auto simp add: invAux_def n_Idle_def n_Idle_st_def n_Idle_st_ref_def)
+lemma n_Idle2Eq:
+  "n_Idle2 N i = n_Idle2_ref N i"
+  by (auto simp add: invAux_def n_Idle_def n_Idle2_def n_Idle2_ref_def)
 
-lemma absIdle2:
+lemma absIdle2Guard:
   assumes "M \<le> N"
   shows
-  "absTransfForm M (pre (n_Idle_st_ref N i)) =
+  "absTransfForm M (pre (n_Idle2_ref N i)) =
     (if i \<le> M then
        IVar (Para ''n'' i) =\<^sub>f Const E
      else
        (\<forall>\<^sub>fj. \<not>\<^sub>f IVar (Para ''n'' j) =\<^sub>f Const C) M \<and>\<^sub>f
        (\<forall>\<^sub>fj. \<not>\<^sub>f IVar (Para ''n'' j) =\<^sub>f Const E) M)"
-  by (auto simp add: assms n_Idle_st_ref_def)
+  by (auto simp add: assms n_Idle2_ref_def)
+
+lemma absIdle2:
+  assumes "M \<le> N"
+  shows "absTransfRule M (n_Idle2_ref N i) =
+         (if i \<le> M then n_Idle i else n_Idle_abs2 M)"
+  unfolding n_Idle_def n_Idle_abs2_def n_Idle2_ref_def using assms by auto
 
 (*
 definition rules_i :: "nat \<Rightarrow> nat \<Rightarrow> rule set" where
